ERT/Stlc/DeBruijn2/Basic.lean
@@ -1,0 +1,69 @@
+import Mathlib.Data.Fin.Tuple.Basic
+
+import ERT.Stlc.DeBruijn2.Syntax
+import ERT.Utils.Wk
+
+namespace Stlc.DeBruijn2
+
+open Term
+open Ty
+
+inductive HasTy: Ctx BaseTy -> Term -> Ty BaseTy -> Type
+| var : (k: Fin Γ.length) -> HasTy Γ (var k.val) (Γ.get k)
+| app : HasTy Γ s (fn A B)
+    -> HasTy Γ t A
+    -> HasTy Γ (app s t) B
+| lam : HasTy (A :: Γ) t B -> HasTy Γ (lam A t) (fn A B)
+| pair : HasTy Γ s A
+    -> HasTy Γ t B
+    -> HasTy Γ (pair s t) (prod A B)
+| let1: HasTy Γ s A
+    -> HasTy (A :: Γ) t B
+    -> HasTy Γ (let1 s t) B
+| let2 : HasTy Γ s (prod A B)
+    -> HasTy (A :: B :: Γ) t C
+    -> HasTy Γ (let2 s t) C
+| case : HasTy Γ s (coprod A B)
+    -> HasTy (A :: Γ) t C
+    -> HasTy (B :: Γ) u C
+    -> HasTy Γ (case s t u) C
+| inl : HasTy Γ s A -> HasTy Γ (inj 0 s) (coprod A B)
+| inr : HasTy Γ s B -> HasTy Γ (inj 1 s) (coprod A B)
+| abort A : HasTy Γ (abort A) A
+
+def HasTy.wk {ρ} {Γ Δ: Ctx BaseTy} {t: Term} {A: Ty BaseTy}
+  (R: WkList ρ Γ Δ): HasTy Δ t A -> HasTy Γ (t.wk ρ) A
+  | var v => R.get_eq v ▸ var (R.toWkNat.app v)
+  | app s t => app (HasTy.wk R s) (HasTy.wk R t)
+  | lam t => lam (HasTy.wk (WkList.lift _ R) t)
+  | pair s t => pair (HasTy.wk R s) (HasTy.wk R t)
+  | let1 s t => let1 (HasTy.wk R s) (HasTy.wk (WkList.lift _ R) t)
+  | let2 s t => let2 (HasTy.wk R s) (HasTy.wk (WkList.lift _ (WkList.lift _ R)) t)
+  | case s t u => case (HasTy.wk R s)
+    (HasTy.wk (WkList.lift _ R) t)
+    (HasTy.wk (WkList.lift _ R) u)
+  | inl s => inl (HasTy.wk R s)
+  | inr s => inr (HasTy.wk R s)
+  | abort A => abort A
+
+def Subst.Valid (σ: Subst) (Γ Δ: Ctx BaseTy)
+    := (k: Fin Δ.length) -> HasTy Γ (σ k.val) (Δ.get k)
+
+def Subst.Valid.lift {σ: Subst} {Γ Δ: Ctx BaseTy}
+    (A: Ty BaseTy) (V: Subst.Valid σ Γ Δ): Subst.Valid σ.lift (A :: Γ) (A :: Δ)
+    := Fin.cons (HasTy.var ⟨0, by simp⟩) (λk => (V k).wk (WkList.wk1 _ _))
+
+def HasTy.subst {σ} {Γ Δ: Ctx BaseTy} {t: Term} {A: Ty BaseTy}
+    (V: Subst.Valid σ Γ Δ): HasTy Δ t A -> HasTy Γ (t.subst σ) A
+    | var v => V v
+    | app s t => app (HasTy.subst V s) (HasTy.subst V t)
+    | lam t => lam (HasTy.subst (V.lift _) t)
+    | pair s t => pair (HasTy.subst V s) (HasTy.subst V t)
+    | let1 s t => let1 (HasTy.subst V s) (HasTy.subst (V.lift _) t)
+    | let2 s t => let2 (HasTy.subst V s) (HasTy.subst ((V.lift _).lift _) t)
+    | case s t u => case (HasTy.subst V s)
+        (HasTy.subst (V.lift _) t)
+        (HasTy.subst (V.lift _) u)
+    | inl s => inl (HasTy.subst V s)
+    | inr s => inr (HasTy.subst V s)
+    | abort A => abort A
